redefined Topic so that it exactly extracts to the roshask definition.

src/shim/Haskell/RoshaskMsg.v
@@ -2,48 +2,19 @@ Require Import String.
 Require Import ExtrHaskellString.
 Require Import ROSCOQ.CoList.
 Require Import RoshaskNodeMonad.
+Require Import RoshaskTopic.
 
 
-Definition TopicName : Type := string.
-
-(** These are streams that can be published/subscribed to/from ROS topics.
-    However, there can be streams which are 
-    only used for intermediate results, or even stremas
-    which have nothing to do with topics.
-    
-    One can think of [ROSStream T] as [Topic IO T] in roshask.
-    Note that the notation [] in comments has nothing to do with lists.
-    These are coqdoc directives to indicate that the thing inside is a code object.
-  *)
-Definition ROSStream (T:Type) := CoList T.
-
-(* Haskell Definition, which doesn't work in Coq, because m may not be positive
-newtype Topic m a = Topic { runTopic :: m (a, Topic m a) } 
-
-CoInductive Topic (m:Type ->Type) `{Monad m} (a:Type) :=
-| CTopic (runTopic : m (a × Topic m a)).
-
-
-Error: Non strictly positive occurrence of "Topic" in
- "m (a × Topic m H H0 H1 H2 a) → Topic m H H0 H1 H2 a". 
-*)
-
-
+(*
 Axiom Chan : Type -> Type.
 Extract Constant Chan "a" => "Control.Concurrent.Chan a".
+*)
 
 Class ROSMsgType (T:Type) :=
   {
-    (* it will be incorrect to remove [Node] (monad) below. If the return type was
-      just [CoList T], Coq's semantics need that it be reduced to either a [cnil]
-      or a [ccons _ _] within a bounded amount of time. Unfortunately, since
-      elements of this "stream" are coming from outside world, we have no control over
-      when things will arrive.       
-      Also, there will be issues with being a function, i.e. equal output for equal topic name.
- *)
-   subscribe : TopicName -> Node (CoList T);
-   publish : TopicName -> CoList T -> Node unit; (*will be mapped to advertize in Roshask*)
-   advertiseNewChan  : TopicName -> Node (Chan T)
+   subscribe : TopicName -> Node (RTopic T);
+   publish : TopicName -> RTopic T -> Node unit (*will be mapped to advertize in Roshask*)
+   (*; advertiseNewChan  : TopicName -> Node (Chan T) *)
 }.
 
 (**roshask will be modified to generate Coq Types for ROS message types. These message types
@@ -53,15 +24,17 @@ On top of these functions, the ROSCoq message handler functionality has been bui
 *)
 
 
-
+(*
 Axiom  publishMsgOnChan: forall {a:Type}, (Chan a) -> a -> Node unit.
 Extract Constant publishMsgOnChan => "Ros.ROSCoqUtil.publishMsgOnChan".
 
 
-Require ExtrHaskellZNum.
-Require Import ZArith.
 
 Axiom publishDelayedMsgOnChan: forall {a:Type}, Z -> (Chan a) -> a -> Node unit.
 Extract Constant publishDelayedMsgOnChan => "Ros.ROSCoqUtil.publishDelayedMsgOnChan".
+ *)
+
+Require ExtrHaskellZNum.
+Require Import ZArith.
 Definition delayResolutionSecInv :  positive := (1000000)%positive. (** depends on the Haskell definition of the function above.*)
 
