src/shim/Haskell/RoshaskNodeMonad.v
@@ -34,27 +34,7 @@ Instance MonadInstanceNodeHaskell : forall nodeEq, @Monad Node nodeEq _ _ :=
   AssumeMonadNodeHaskell.
 
 
-Require Import CoList.
 
-(** this is not a pure computation. the final result depends on not just
-   the values of the 2 streams, but when items in the streams arrived*)
-Axiom asapMerge :  forall {A:Type}, CoList A -> CoList A -> Node (CoList A).
-Extract Constant asapMerge => "Ros.ROSCoqUtil.asapMergeCoList".
-
-(** lack of productivity is the only thing in the way of this being a pure function.
-    We never know if we will keep getting empty lists in input forever. So the
-    returned [CoList] cannot be evaluated to either [cnil] or [ccons] in bounded amount 
-    of time. Hence we put this computation in the Node monad. 
-   Node (CoList A) is an abstract type (neither inductive, nor coinductive).
-
-Not needed anymore?
-*)
-Axiom flattenCoListList :  forall {A:Type}, CoList (list A)  -> Node (CoList A).
-Extract Constant flattenCoListList => "(\ll -> GHC.Base.return (Prelude.concat ll))".
-(** recall that [CoList T] extracts to Haskell as [T]. *)
-
-Axiom coFoldLeft: forall {a b:Type}, (a-> b ->Node a)-> CoList b -> a -> Node a.
-Extract Constant coFoldLeft => "Ros.ROSCoqUtil.coFoldLeft".
 
 
 
