src/shim/Haskell/RoshaskTopic.v
@@ -1,0 +1,49 @@
+Require Import String.
+Require Import ExtrHaskellString.
+Require Import RoshaskNodeMonad.
+
+
+Definition TopicName : Type := string.
+
+Axiom RTopic : Type -> Type.
+(** TODO: generalize over the IO monad. *)
+
+Extract Constant RTopic "a" => "Ros.Node.Topic GHC.Base.IO a".
+
+(* Haskell Definition, which doesn't work in Coq, because m may not be positive
+newtype Topic m a = Topic { runTopic :: m (a, Topic m a) } 
+
+CoInductive Topic (m:Type ->Type) `{Monad m} (a:Type) :=
+| CTopic (runTopic : m (a × Topic m a)).
+
+
+Error: Non strictly positive occurrence of "Topic" in
+ "m (a × Topic m H H0 H1 H2 a) → Topic m H H0 H1 H2 a". 
+*)
+
+
+(** TODO: make it an instance of functior*)
+Axiom tmap : forall {A B :Type}, (A->B) -> RTopic A -> RTopic B.
+Extract Constant tmap  => "fmap".
+
+Axiom tfilter : forall {A B: Type} (f: A -> bool)
+                  (g: forall (a:A) {pr: f a = true}, B), RTopic A -> RTopic B.
+Extract Constant tfilter  => "\f g l -> fmap g (Ros.Topic.filter f l)".
+
+(** this is not a pure computation. the final result depends on not just
+   the values of the 2 streams, but when items in the streams arrived*)
+Axiom asapMerge :  forall {A:Type}, (RTopic A) -> (RTopic A) -> (RTopic A).
+Extract Constant asapMerge => "Ros.Topic.Util.merge".
+
+Axiom flattenTL : forall {A:Type}, (RTopic (list A)) -> (RTopic A).
+Extract Constant flattenTL => "Ros.ROSCoqUtil.flattenTL".
+
+Axiom foldMapL : forall {s a b :Type}, s -> (s -> a -> (b * s)) -> RTopic a -> RTopic b.
+Extract Constant foldMapL => "Ros.ROSCoqUtil.foldMapL".
+
+
+
+
+
+
+
